\documentclass[a4paper,10pt]{article}

\usepackage[
	left=1cm,right=1cm,top=1cm,bottom=2cm,
    papersize={250mm,350mm}
]{geometry}


\usepackage[english]{babel}
\usepackage[utf8]{inputenc}

\usepackage{amsmath}
\usepackage{amssymb}
\usepackage{physics}
\usepackage{dsfont}

\usepackage[squaren]{SIunits}
\usepackage{graphicx}
\usepackage{xcolor}

\newcommand{\mi}{\mathrm{i}}
\newcommand{\suml}{\sum\limits}
\newcommand{\prodl}{\prod\limits}
\newcommand{\intl}{\int\limits}


\begin{document}

\begin{align}
    \vb{E}
    &=
    -2\phi_0 x\vb{e}_x
\\
    \phi
    &=
    -
    \vb{r}
    \cdot
    \intl_0^1
    \dd{u}
    \vb{E}(u\vb{r},t)
    =
    2\phi_0
    x^2
    \intl_0^1
    \dd{u}
    u
    =
    \phi_0
    x^2
\end{align}


\begin{align}
    \vb{B}
    &=
    B{e}_z
\\
    \vb{A}
    &=
    -
    \vb{r}
    \times
    \intl_0^1
    \dd{u}
    u
    \vb{B}(u\vb{r},t)
    =
    \frac{B}{2}
    \pmqty{
        -y\\x\\0
    }
\end{align}

\begin{align}
    \vb{A}
    &\to
    \vb{A}
    +
    \nabla
    \Lambda
    =
    B
    \pmqty{
        0\\x\\0
    }
\\
    \Lambda
    &=
    \frac{B}{2}
    xy
\\
    \phi^\prime
    &\to
    \phi-\partial_t \Lambda=\phi
\end{align}

\begin{align}
    \hat{H}
    &=
    \frac{1}{2m}
    (\hat{p}_x^2+\hat{p}_z^2)
    +
    \frac{1}{2m}
    (\hat{p}_y-qB\hat{x})^2
    +
    \phi_0
    \hat{x}^2
\\
    &=
    \frac{1}{2m}
    (\hat{p}_x^2+\hat{p}_y^2+\hat{p}_z^2)
    -
    \frac{qB}{m}
    \hat{x}
    \hat{p}_y
    +
    \pqty{
	    \frac{q^2B^2}{2m}
	    +
    		\phi_0
    	}
    \hat{x}^2
\end{align}


\begin{align}
    \bqty{
        \hat{H}
        ,
        \hat{p}_z
    }
    &=
    \bqty{
        \hat{H}
        ,
        \hat{p}_y
    }
    =
    0
\\
    \hat{p}_z
    &\to
    p_z
    ,\quad
    \hat{p}_y
    \to
    p_y
    ,\quad
    \hat{p}_x
    \to
    -\mi\hbar\partial_x
\\
    \psi(x,y,z)
    &=
    e^{
        \frac{\mi}{\hbar}
        (yp_y+zp_z)
    }
    \chi(x)
\end{align}


$\omega_c=\sqrt{\frac{q^2 B^2}{m^2}+2\frac{\phi_0}{m}}$



\begin{align}
	\hat{H}    
    &=
    \frac{p_y^2+p_z^2}{2m}
	-
    \frac{\hbar^2}{2m}    
    \partial_x^2
    -
    \frac{qBp_y}{m}
    x
    +
    \frac{1}{2}
    m\omega_c^2
    x^2
\\
	&=
    \frac{p_y^2+p_z^2}{2m}
	-
    \frac{\hbar^2}{2m}    
    \partial_x^2
	+
    \frac{1}{2}
    m\omega_c^2
	\pqty{
		x
		-
		\frac{qBp_y}{m^2\omega_c^2}
	}^2
	-
	\frac{q^2 B^2 p_y^2}{2m^3\omega_c^2}
\end{align}

$\xi = x-x_0=x-\frac{qBp_y}{m^2\omega_c^2}$, $C=\frac{q^2 B^2 p_y^2}{2m^3\omega_c^2}$

\begin{align}
	\hat{H}
	&=
    \frac{p_y^2+p_z^2}{2m}
	-
	C
	-
    \frac{\hbar^2}{2m}    
    \partial_\xi^2
	+
	\frac{1}{2}
	m
	\omega_c^2
	\xi^2
\\
	\hat{H}_1
	&=	
	\hat{H}-\hat{H}_0
	=
	-
    \frac{\hbar^2}{2m}    
    \partial_\xi^2
	+
	\frac{1}{2}
	m
	\omega_c^2
	\xi^2
\end{align}


\begin{align}
	E_1
	\chi(\xi)
	&=
	\hat{H}_1
	\chi(\xi)
\\
	\chi_n(\xi)
	&=
	N_n
	e^{-\frac{m\omega_c}{2\hbar}\xi^2}
	H_n\pqty{
		\sqrt{
			\frac{m\omega_c}{\hbar}	
		}
		\xi
	}
\end{align}

$N_n=\frac{1}{\sqrt{2^n n!}}\pqty{\frac{m\omega_c}{\pi\hbar}}^{\frac{1}{4}}$

\begin{align}
	\psi_{n,p_y,p_z}
	&=
	e^{\frac{\mi}{\hbar}(yp_y+zp_z-Ct)}
	\chi_{n,p_y}
	(x-x_0)
\\
	\chi_{n,p_y}
	(x-x_0)
	&=
	N_n
	\exp
	\pqty{
		-
		\frac{m\omega_c}{2\hbar}
		\pqty{
			x-\frac{qBp_y}{m^2\omega_c^2}		
		}^2
	}
	H_n\pqty{
		\sqrt{
			\frac{m\omega_c}{\hbar}	
		}
		\pqty{
			x-\frac{qBp_y}{m^2\omega_c^2}		
		}
	}
\end{align}

\begin{align}
	\psi_{0,p_y,p_z}
	(x,y,z)
	&=
	\pqty{
		\frac{m\omega_c}{\pi\hbar}
	}^{\frac{1}{4}}
	\exp
	\pqty{
		-
		\frac{m\omega_c}{2\hbar}
		\pqty{
			x-\frac{qBp_y}{m^2\omega_c^2}
		}^2
		+
		\frac{\mi}{\hbar}
		p_y y
		+
		\frac{\mi}{\hbar}
		p_z z
		-
		\frac{\mi}{\hbar}
		Ct
	}
\\
	\abs{
		\psi_{0,p_y,p_z}
		(x,y,z)
	}^2
	&=
	\sqrt{
		\frac{m\omega_c}{\pi\hbar}
	}
	\exp
	\pqty{
		-
		\frac{m\omega_c}{\hbar}
		\pqty{
			x-\frac{qBp_y}{m^2\omega_c^2}
		}^2
	}	
\end{align}


\begin{align}
	E
	&=
	E_0
	+
	E_1^{(n)}
	=
    \frac{p_y^2+p_z^2}{2m}
	-
	C
	+
	\hbar\omega_c
	(n+\frac{1}{2})
\\
	&=
    \frac{p_y^2+p_z^2}{2m}
	-
	\frac{q^2 B^2 p_y^2}
	{
		2m^3
		\pqty{\frac{q^2 B^2}{m^2}+2\frac{\phi_0}{m}}
	}
	+
	\hbar
	\sqrt{\frac{q^2 B^2}{m^2}+2\frac{\phi_0}{m}}
	\pqty{n+\frac{1}{2}}
\end{align}


\begin{align}
	\vb{A}^\prime
	&=
	\vb{A}
	+
	\nabla\Lambda
	=
	B\pmqty{0\\x\\0}
	-
	B\pmqty{0\\x_1\\0}
\\
	\Lambda
	&=
	-Bx_1 y
\\
	\phi^\prime
	&=
	\phi
	-
	\partial_t
	\Lambda
	=
	\phi
\end{align}


\begin{align}
    \hat{H}^\prime
    &=
    \frac{1}{2m}
    (\hat{p}_x^2+\hat{p}_z^2)
    +
    \frac{1}{2m}
    (\hat{p}_y-qB\hat{x}+qBx_1)^2
    +
    \phi_0
    \hat{x}^2
\\
    &=
    \frac{1}{2m}
    (\hat{p}_x^2+\hat{p}_y^2+\hat{p}_z^2)
    -
    \pqty{
	    \frac{qB}{m}
    		\hat{p}_y
    		+
	    \frac{q^2B^2}{m}
    		x_1
    }
	\hat{x}
    +
    \pqty{
	    \frac{q^2B^2}{2m}
	    +
    		\phi_0
    	}
    \hat{x}^2
    +
    \frac{qB}{m}
    \hat{p}_y
    x_1
    +
    \frac{q^2B^2}{2m}
    x_1^2
\end{align}

$\omega_c=\sqrt{\frac{q^2 B^2}{m^2}+2\frac{\phi_0}{m}}$

\begin{align}
	\hat{H}^\prime  
    &=
    \frac{p_y^2+p_z^2}{2m}
	-
    \frac{\hbar^2}{2m}    
    \partial_x^2
    -
    \pqty{
	    \frac{qB}{m}
    		p_y
    		+
	    \frac{q^2B^2}{m}
    		x_1
    }
    x
    +
    \frac{1}{2}
    m\omega_c^2
    x^2
    +
    \frac{qB}{m}
    p_y
    x_1
    +
    \frac{q^2B^2}{2m}
    x_1^2
\\
	&=
    \frac{p_y^2+p_z^2}{2m}
	-
    \frac{\hbar^2}{2m}    
    \partial_x^2
	+
    \frac{1}{2}
    m\omega_c^2
	\pqty{
		x
		-
		\frac{qBp_y}{m^2\omega_c^2}
		-
		\frac{q^2 B^2}{m^2\omega_c^2}
		x_1
	}^2
	-
	\frac{qBp_y}{2m^2\omega_c^2}
	-
	\frac{q^2 B^2}{2m^2\omega_c^2}x_1
    +
    \frac{qB}{m}
    p_y
    x_1
    +
    \frac{q^2B^2}{2m}
    x_1^2
\end{align}

$\zeta = x-x_0^\prime=x-\frac{qBp_y}{m^2\omega_c^2}-\frac{q^2 B^2}{m^2\omega_c^2}x_1$,
$C^\prime=\frac{qBp_y}{2m^2\omega_c^2}+\frac{q^2 B^2}{2m^2\omega_c^2}x_1-\frac{qB}{m}p_y x_1-\frac{q^2B^2}{2m}x_1^2$

\begin{align}
	\hat{H}^\prime
	&=
    \frac{p_y^2+p_z^2}{2m}
	-
	C^\prime
	-
    \frac{\hbar^2}{2m}    
    \partial_\zeta^2
	+
	\frac{1}{2}
	m
	\omega_c^2
	\zeta^2
\\
	\hat{H}_1
	&=	
	\hat{H}-\hat{H}_0
	=
	-
    \frac{\hbar^2}{2m}    
    \partial_\zeta^2
	+
	\frac{1}{2}
	m
	\omega_c^2
	\zeta^2
\end{align}

$N_n=\frac{1}{\sqrt{2^n n!}}\pqty{\frac{m\omega_c}{\pi\hbar}}^{\frac{1}{4}}$

\begin{align}
	\psi^\prime_{n,p_y,p_z}
	&=
	e^{\frac{\mi}{\hbar}(yp_y+zp_z-C^\prime t)}
	\chi^\prime_{n,p_y}
	(x-x_0^\prime)
\\
	\chi^\prime_{n,p_y}
	(x-x_0^\prime)
	&=
	N_n
	\exp
	\pqty{
		-
		\frac{m\omega_c}{2\hbar}
		\pqty{
			x-\frac{qBp_y}{m^2\omega_c^2}-\frac{q^2 B^2}{m^2\omega_c^2}x_1
		}^2
	}
	H_n\pqty{
		\sqrt{
			\frac{m\omega_c}{\hbar}	
		}
		\pqty{
			x-\frac{qBp_y}{m^2\omega_c^2}-\frac{q^2 B^2}{m^2\omega_c^2}x_1
		}
	}
\end{align}

\begin{align}
	\psi^\prime_{0,p_y,p_z}
	(x,y,z)
	&=
	\pqty{
		\frac{m\omega_c}{\pi\hbar}
	}^{\frac{1}{4}}
	\exp
	\pqty{
		-
		\frac{m\omega_c}{2\hbar}
		\pqty{
			x-\frac{qBp_y}{m^2\omega_c^2}-\frac{q^2 B^2}{m^2\omega_c^2}x_1
		}^2
		+
		\frac{\mi}{\hbar}
		p_y y
		+
		\frac{\mi}{\hbar}
		p_z z
		-
		\frac{\mi}{\hbar}
		C^\prime t
	}
\\
	\abs{
		\psi^\prime_{0,p_y,p_z}
		(x,y,z)
	}^2
	&=
	\sqrt{
		\frac{m\omega_c}{\pi\hbar}
	}
	\exp
	\pqty{
		-
		\frac{m\omega_c}{\hbar}
		\pqty{
			x
			-\frac{qBp_y}{m^2\omega_c^2}
			-\frac{q^2 B^2}{m^2\omega_c^2}x_1
		}^2
	}
	\neq
	\abs{
		\psi_{0,p_y,p_z}
		(x,y,z)
	}^2
\\
	p_y
	&\neq
	p_y^\prime
\end{align}

\newpage

\begin{align}
    \vb{E}
    &=
    -2\phi_{0x} x\vb{e}_x
    -2\phi_{0y} y\vb{e}_y
\\
    \phi
    &=
    -
    \vb{r}
    \cdot
    \intl_0^1
    \dd{u}
    \vb{E}(u\vb{r},t)
    =
    2
    (
    		\phi_{0x}
    		x^2
    		+
    		\phi_{0y}
    		y^2
    	)
    \intl_0^1
    \dd{u}
    u
    =
    	\phi_{0x}
    	x^2
    	+
    	\phi_{0y}
    	y^2
\end{align}


\begin{align}
    \vb{B}
    &=
    B{e}_z
\\
    \vb{A}
    &=
    -
    \vb{r}
    \times
    \intl_0^1
    \dd{u}
    u
    \vb{B}(u\vb{r},t)
    =
    \frac{B}{2}
    \pmqty{
        -y\\x\\0
    }
\end{align}

\begin{align}
    \vb{A}
    &\to
    \vb{A}
    +
    \nabla
    \Lambda
    =
    B
    \pmqty{
        0\\x\\0
    }
\\
    \Lambda
    &=
    \frac{B}{2}
    xy
\\
    \phi^\prime
    &\to
    \phi-\partial_t \Lambda=\phi
\end{align}

\begin{align}
    \hat{H}
    &=
    \frac{1}{2m}
    (\hat{p}_x^2+\hat{p}_z^2)
    +
    \frac{1}{2m}
    (\hat{p}_y-qB\hat{x})^2
    +
    \phi_{0x}
    \hat{x}^2
    +
    \phi_{0y}
    \hat{y}^2
\\
    &=
    \frac{1}{2m}
    (\hat{p}_x^2+\hat{p}_y^2+\hat{p}_z^2)
    -
    \frac{qB}{m}
    \hat{x}
    \hat{p}_y
    +
    \pqty{
	    \frac{q^2B^2}{2m}
	    +
    		\phi_{0x}
    	}
    \hat{x}^2
    +
    \phi_{0y}
    \hat{y}^2
\end{align}


\begin{align}
    \bqty{
        \hat{H}
        ,
        \hat{p}_z
    }
    &=
    0
\\
    \hat{p}_z
    &\to
    p_z
    ,\quad
    \hat{p}_y
    \to
    -\mi\hbar\partial_y
    ,\quad
    \hat{p}_x
    \to
    -\mi\hbar\partial_x
\\
    \psi(x,y,z)
    &=
    e^{
        \frac{\mi}{\hbar}
        zp_z
    }
    \chi(x,y)
\end{align}

$\omega_c=\sqrt{\frac{q^2 B^2}{m^2}+2\frac{\phi_{0x}}{m}}$



\begin{align}
	\hat{H}    
    &=
    \frac{p_z^2}{2m}
    	-
    \frac{\hbar^2}{2m}    
    \partial_y^2
    +
    \phi_{0y}
    y^2
	-
    \frac{\hbar^2}{2m}    
    \partial_x^2
    -
    \frac{qB}{m}
    x
    \partial_y
    +
    \frac{1}{2}
    m\omega_c^2
    x^2
\end{align}

\end{document} 
